AP/AP/Symmetry/Basic.lean
@@ -1,0 +1,3 @@
+import AP.AP.Symmetry.Defs
+
+namespace AP
