AP/AP/Symmetry/Defs.lean
@@ -1,0 +1,22 @@
+import AP.AP.Determinacy
+
+namespace AP
+
+def symFnState (f : PointZ → PointZ) (s : State) : State where
+  pw := s.pw
+  taken := s.taken.map f
+  aPos := f s.aPos
+  aTurn := s.aTurn
+  hist := s.hist.map f
+
+#check 0 #exit
+
+def mkSym (f f' : PointZ → PointZ) (h₁ : Inverse f f') : sys.Symmetry where
+  fs := symFnState f
+  fs' := symFnState f'
+  ft := f
+  ft' := f'
+  wf :=
+    { h_fs := by
+        simp
+    }
